p256: mv ith_bit to Hacl.Impl.P256.PointMul

code/ecdsap256/Hacl.Impl.P256.Bignum.fst
@@ -15,14 +15,6 @@ module SN = Hacl.Spec.Bignum
 
 #set-options "--z3rlimit 50 --fuel 0 --ifuel 0"
 
-let scalar_bit #buf_type s n =
-  let h0 = ST.get () in
-  mod_mask_lemma ((Lib.Sequence.index (as_seq h0 s) (v n / 8)) >>. (n %. 8ul)) 1ul;
-  assert_norm (1 = pow2 1 - 1);
-  assert (v (mod_mask #U8 #SEC 1ul) == v (u8 1));
-  to_u64 ((s.(n /. 8ul) >>. (n %. 8ul)) &. u8 1)
-
-
 ///  Create a bignum
 
 let bn_make_u64_4 a0 a1 a2 a3 res =
